{
 "cells": [
  {
   "cell_type": "code",
   "execution_count": null,
   "id": "a00c9098-de4f-471f-90a1-b66b30ba1a12",
   "metadata": {},
   "outputs": [],
   "source": [
    "#1.Find the value of T(2) for the recurrence relation T(n) = 3T(n-1) + 12n, given that T(0)=5\n",
    "T(n) =3T(n-1) + 12n\n",
    "T(2) = 3T(2-1) + 12(2)\n",
    "T(2) = 3T(1) + 12(2) ------>(1)\n",
    "To find the value of T(1)\n",
    "T(1) = 3T(1-1) +12(1)\n",
    "T(1) = 3T(0) + 12(1) ------>(2)\n",
    "substute T(0) = 5 in equation(2)\n",
    "T(1) = 3*5 + 12\n",
    "T(1) =15+12 = 27\n",
    "After that T(1) value substitute in equation 1\n",
    "\n",
    "T(2) =3(27)+24\n",
    "T(2) =81+24\n",
    "T(2) = 105\n",
    "  Therefore T(2) = 105  "
   ]
  },
  {
   "cell_type": "code",
   "execution_count": null,
   "id": "edcfc45d-512e-4d40-be83-7a5fbf7eb1b5",
   "metadata": {},
   "outputs": [],
   "source": [
    "#2. Given a recurrence relation, solve it using the substitution method:\n",
    "\n",
    "a. T(n) = T(n-1) + c\n",
    "\n",
    "Lets expand T(n - 1)cc\n",
    "T(n)=T(n-1 -1) +c\n",
    "T(n)=(T(n-2)+c)+c\n",
    "T(n)=T(n-2)+2c\n",
    "T(n)=T(n-3)+3c\n",
    "|\n",
    "|\n",
    "T(n)=T(1)+(n-1)c\n",
    "so, the solution is T(n) = T(1) + (n-1)c\n",
    "\n",
    "b. T(n) = 2T(n/2) + n\n",
    "Assume that T(k) = ck-d for constants c and d\n",
    "Now,substitue this assumption into the recurrence releation\n",
    "T(k) = 2(c(n/2)-d)+n\n",
    "T(k) = 2cn/2-2d+n\n",
    "T(k) = cn-2d+n\n",
    "now, set the equation to the assumed form \n",
    "cn-2d+n = ck-d\n",
    "solve for c and d\n",
    "c = 2\n",
    "d = n\n",
    "so,the solution is T(n)=2n-n = n\n",
    "\n",
    "c.T(n) = 2T(n/2) + c\n",
    "\n",
    "Assume that T(k) = ck for constant c\n",
    "T(n) = 2T(n/2) + c\n",
    "T(n) = 2c(n/2) + c\n",
    "T(n) = 2cn/2 + c\n",
    "T(n) = cn + c\n",
    "so, the solution is T(n) = cn + c\n",
    "d.T(n)=T(n/2)+c\n",
    "\n",
    "Assume that T(k) =ck for some constant c\n",
    "T(n) = c(n/2) + c\n",
    "T(n) = cn/2 + c\n",
    "so, the solution is T(n) = cn/2 + csss"
   ]
  },
  {
   "cell_type": "code",
   "execution_count": null,
   "id": "2ec1836a-5f89-403b-8451-a2a220fc7121",
   "metadata": {},
   "outputs": [],
   "source": [
    "#3. Given a recurrence relation, solve it using the recursive tree approach:\n",
    "\n",
    "a. T(n) = 2T(n-1) +1\n",
    "first,Draw the recursive tree for the recurrence relation \n",
    "                     \n",
    "                      T(n)\n",
    "                     /   \\\n",
    "                 T(n-1)   T(n-1)\n",
    "                   / \\     / \\\n",
    "               T(n-2) T(n-2) T(n-2) T(n-2)\n",
    "                / \\    / \\    / \\    / \\\n",
    "           T(n-3) ... T(n-3) T(n-3) T(n-3)\n",
    "At each Level The Recurrence branches into two subproblems of  size n - 1,and the work done at each level is 1.\n",
    "The total number of levels in recursive tree is n. Lets count the work done at each level.\n",
    "Level 0 = 1 work\n",
    "Level 1 = 2 work\n",
    "Level 2 = 2^2 work\n",
    "Level 3 = 2^3 work\n",
    ".....\n",
    "Level k = 2^k work\n",
    "The total work done is the sum of these geometric series\n",
    "1 + 2 + 2^2 + 2^3 +....+ 2^(n-1) = 2^n -1\n",
    "The solution is T(n) = 2^n - 1\n",
    "\n",
    "b. T(n) = 2T(n/2) + n\n",
    "\n",
    "                   T(n)\n",
    "                   / \\\n",
    "             2T(n/2) 2T(n/2)\n",
    "              / \\      / \\\n",
    "          T(n/4) ... T(n/4) T(n/4) ...\n",
    "\n",
    "At each level, the recurrence branches into two subproblems of size n/2 and the work done by each level is n.\n",
    "The total number of recursion tree level is log(n) base 2.now counts the work done at each level.\n",
    "Level 0 = n work\n",
    "Level 1 = 2.n/2 = n work\n",
    "Level 2 = 2^2.n/2^2 = n works\n",
    "Level 3 = 2^3.n/2^3 = n works\n",
    "..............\n",
    "Level k = 2^k.n/2^k = n works\n",
    "The total work done is the product of the work at each level and the number of nodes at each level:\n",
    "n.log(n) Base 2\n",
    "\n",
    "Therefore , the solution is T(n) = n.log base2(n)\n",
    "    "
   ]
  }
 ],
 "metadata": {
  "kernelspec": {
   "display_name": "Python 3 (ipykernel)",
   "language": "python",
   "name": "python3"
  },
  "language_info": {
   "codemirror_mode": {
    "name": "ipython",
    "version": 3
   },
   "file_extension": ".py",
   "mimetype": "text/x-python",
   "name": "python",
   "nbconvert_exporter": "python",
   "pygments_lexer": "ipython3",
   "version": "3.10.8"
  }
 },
 "nbformat": 4,
 "nbformat_minor": 5
}
